only need ins_RB

SF_RB.v
@@ -7,62 +7,63 @@ Require Import Lia.
 
 Definition key := nat.
 Inductive color := Red | Black.
-Inductive tree (V : Type) : Type :=
-| E : tree V
-| T : color -> tree V -> key -> V -> tree V -> tree V.
-Arguments E {V}.
-Arguments T {V}.
-Definition empty_tree (V : Type) : tree V :=
+
+Inductive tree  :=
+| E : tree
+| T : color -> tree -> nat -> tree -> tree.
+
+Definition empty_tree : tree :=
   E.
 
-Definition balance
-           {V : Type} (c : color) (t1 : tree V) (k : key) (vk : V)
-           (t2 : tree V) : tree V :=
+(*   Arguments E {V}.
+Arguments T {V}. *)
+
+Definition balance (c : color) (t1 : tree) (k : nat) (t2 : tree) : tree :=
   match c with
-  | Red => T Red t1 k vk t2
-  | _ => match t1 with
-        | T Red (T Red a x vx b) y vy c =>
-            T Red (T Black a x vx b) y vy (T Black c k vk t2)
-        | T Red a x vx (T Red b y vy c) =>
-            T Red (T Black a x vx b) y vy (T Black c k vk t2)
-        | _ => match t2 with
-              | T Red (T Red b y vy c) z vz d =>
-                  T Red (T Black t1 k vk b) y vy (T Black c z vz d)
-              | T Red b y vy (T Red c z vz d) =>
-                  T Red (T Black t1 k vk b) y vy (T Black c z vz d)
-              | _ => T Black t1 k vk t2
-              end
-        end
+  | Red => T Red t1 k t2
+  | Black => 
+      match t1 with
+      | T Red (T Red a x b) y c =>
+          T Red (T Black a x b) y (T Black c k t2)
+      | T Red a x (T Red b y c) =>
+          T Red (T Black a x b) y (T Black c k t2)
+      | _ => 
+          match t2 with
+          | T Red (T Red b y c) z d =>
+              T Red (T Black t1 k b) y (T Black c z d)
+          | T Red b y (T Red c z d) =>
+              T Red (T Black t1 k b) y (T Black c z d)
+          | _ => T Black t1 k t2
+          end
+      end
   end.
-Fixpoint ins {V : Type} (x : key) (vx : V) (t : tree V) : tree V :=
+Fixpoint ins (x : nat) (t : tree) : tree :=
   match t with
-  | E => T Red E x vx E
-  | T c a y vy b => if ltb x y then balance c (ins x vx a) y vy b
-                   else if ltb y x then balance c a y vy (ins x vx b)
-                        else T c a x vx b
+  | E => T Red E x E
+  | T c a y b => 
+      if ltb x y then balance c (ins x a) y b
+      else if ltb y x then balance c a y (ins x b)
+      else T c a x b
   end.
-Definition make_black {V : Type} (t : tree V) : tree V :=
+Definition make_black (t : tree) : tree :=
   match t with
   | E => E
-  | T _ a x vx b => T Black a x vx b
+  | T _ a vx b => T Black a vx b
   end.
-Definition insert {V : Type} (x : key) (vx : V) (t : tree V) :=
-  make_black (ins x vx t).
+Definition insert (vx : nat) (t : tree) :=
+  make_black (ins vx t).
 
-
-
-Fixpoint elements_aux {V : Type} (t : tree V) (acc: list (key * V))
-  : list (key * V) :=
+(* Fixpoint elements_aux (t : tree) (acc : list nat) : list nat :=
   match t with
   | E => acc
-  | T _ l k v r => elements_aux l ((k, v) :: elements_aux r acc)
+  | T _ l k r => elements_aux l (k :: elements_aux r acc)
   end.
 
-Definition elements {V : Type} (t : tree V) : list (key * V) :=
+Definition elements (t : tree) : list nat :=
   elements_aux t [].
-
-Lemma ins_not_E : forall (V : Type) (x : key) (vx : V) (t : tree V),
-    ins x vx t <> E.
+ *)
+Lemma ins_not_E : forall (vx : nat) (t : tree),
+    ins vx t <> E.
 Proof.
   intros. destruct t; simpl.
   - discriminate.
@@ -70,54 +71,57 @@ Proof.
     repeat
       match goal with
       | |- (if ?x then _ else _) <> _ => destruct x
-      | |- match ?c with Red => _ | Black => _ end <> _=> destruct c
-      | |- match ?t with E => _ | T _ _ _ _ _ => _ end <> _=> destruct t
-      | |- T _ _ _ _ _ <> E => discriminate
+      | |- match ?c with Red => _ | Black => _ end <> _ => destruct c
+      | |- match ?t with E => _ | T _ _ _ _ => _ end <> _ => destruct t
+      | |- T _ _ _ _ <> E => discriminate
       end.
 Qed.
 
 
-Fixpoint ForallT {V : Type} (P: nat -> V -> Prop) (t : tree V) : Prop :=
+Fixpoint ForallT (P: nat -> Prop) (t : tree) : Prop :=
   match t with
   | E => True
-  | T c l k v r => P k v /\ ForallT P l /\ ForallT P r
+  | T c l k r => P k /\ ForallT P l /\ ForallT P r
   end.
-Inductive BST {V : Type} : tree V -> Prop :=
+
+Inductive BST : tree -> Prop :=
 | ST_E : BST E
-| ST_T : forall (c : color) (l : tree V) (k : key) (v : V) (r : tree V),
-    ForallT (fun k' _ => k' < k) l ->
-    ForallT (fun k' _ => k' > k) r ->
+| ST_T : forall (c : color) (l : tree) (k : nat) (r : tree),
+    ForallT (fun k' => k' < k) l ->
+    ForallT (fun k' => k' > k) r ->
     BST l ->
     BST r ->
-    BST (T c l k v r).
-Lemma empty_tree_BST : forall (V : Type), BST (@empty_tree V).
+    BST (T c l k r).
+Lemma empty_tree_BST : forall (V : Type), BST (empty_tree).
 
 Proof.
   unfold empty_tree. constructor.
 Qed.
 
 
-Lemma ForallT_imp : forall (V : Type) (P Q : nat -> V -> Prop) t,
+Lemma ForallT_imp : forall (P Q : nat -> Prop) t,
     ForallT P t ->
-    (forall k v, P k v -> Q k v) ->
+    (forall k, P k -> Q k) ->
     ForallT Q t.
 Proof.
   induction t; intros.
   - auto.
   - destruct H as [? [? ?]]. repeat split; auto.
 Qed.
-Lemma ForallT_greater : forall (V : Type) (t : tree V) (k k0 : key),
-    ForallT (fun k' _ => k' > k) t ->
+
+Lemma ForallT_greater : forall (t : tree) (k k0 : nat),
+    ForallT (fun k' => k' > k) t ->
     k > k0 ->
-    ForallT (fun k' _ => k' > k0) t.
+    ForallT (fun k' => k' > k0) t.
 Proof.
   intros. eapply ForallT_imp; eauto.
   intros. simpl in H1. lia.
 Qed.
-Lemma ForallT_less : forall (V : Type) (t : tree V) (k k0 : key),
-    ForallT (fun k' _ =>  k' <  k) t ->
-    k <  k0 ->
-    ForallT (fun k' _ =>  k' <  k0) t.
+
+Lemma ForallT_less : forall (t : tree) (k k0 : nat),
+    ForallT (fun k' => k' < k) t ->
+    k < k0 ->
+    ForallT (fun k' => k' < k0) t.
 Proof.
   intros; eapply ForallT_imp; eauto.
   intros. simpl in H1. lia.
@@ -125,170 +129,141 @@ Qed.
 
 Ltac inv H := inversion H; subst; clear H.
 
-Lemma balance_BST: forall (V : Type) (c : color) (l : tree V) (k : key)
-                     (v : V) (r : tree V),
-    ForallT (fun k' _ => ( k') < ( k)) l ->
-    ForallT (fun k' _ => ( k') > ( k)) r ->
+Lemma balance_BST: forall (c : color) (l : tree)
+                     (v : nat) (r : tree),
+    ForallT (fun k' => ( k') < ( v)) l ->
+    ForallT (fun k' => ( k') > ( v)) r ->
     BST l ->
     BST r ->
-    BST (balance c l k v r).
+    BST (balance c l v r).
 Proof.
   intros. unfold balance.
   repeat
     match goal with
-    | H: ForallT _ (T _ _ _ _ _) |- _ => destruct H as [? [? ?] ]
-    | H: BST (T _ _ _ _ _) |- _ => inv H
-    | |- BST (T _ _ _ _ _) => constructor
+    | H: ForallT _ (T _ _ _ _) |- _ => destruct H as [? [? ?] ]
+    | H: BST (T _ _ _ _) |- _ => inv H
     | |- BST (match ?c with Red => _ | Black => _ end) => destruct c
-    | |- BST (match ?t with E => _ | T _ _ _ _ _ => _ end) => destruct t
-    | |- ForallT _ (T _ _ _ _ _) => repeat split
+    | |- BST (match ?t with E => _ | T _ _ _ _ => _ end) => destruct t
+    | |- BST (T _ _ _ _) => constructor
+    | |- ForallT _ (T _ _ _ _) => repeat split
     end;
     auto; try lia.
-  (* all: t applies t to every subgoal. *)
   all: try eapply ForallT_greater; try eapply ForallT_less; eauto; try lia.
 Qed.
 
-Lemma balanceP : forall (V : Type) (P : key -> V -> Prop) (c : color) (l r : tree V)
-                   (k : key) (v : V),
+Lemma balanceP : forall (P : nat -> Prop) (c : color) (l r : tree)
+                        (v : nat),
     ForallT P l ->
     ForallT P r ->
-    P k v ->
-    ForallT P (balance c l k v r).
+    P v ->
+    ForallT P (balance c l v r).
 Proof.
   intros.
   unfold balance.
   repeat match goal with
 
 (* If we know P holds for a node, it holds for the key and subtrees. *)
-  | H: ForallT _ (T _ _ _ _ _) |- _ => destruct H as [? [? ?]]
+  | H: ForallT _ (T _ _ _ _) |- _ => destruct H as [? [? ?]]
   
   
 (*  Destruct the variables being matched on inside 'balance'. *)
   | |- ForallT _ (match ?c with Red => _ | Black => _ end) => destruct c
-  | |- ForallT _ (match ?t with E => _ | T _ _ _ _ _ => _ end) => destruct t
+  | |- ForallT _ (match ?t with E => _ | T _ _ _ _ => _ end) => destruct t
   
   (* 3. Solve the Goal: 
         The result is always a T node. Split the ForallT goal into its 3 parts. *)
-  | |- ForallT _ (T _ _ _ _ _) => repeat split
+  | |- ForallT _ (T _ _ _ _) => repeat split
   end;
   auto.
 Qed.
 
 
-Lemma insP : forall (V : Type) (P : key -> V -> Prop) (t : tree V) (k : key) (v : V),
+Lemma insP : forall (P : nat -> Prop) (t : tree) (v : nat),
     ForallT P t ->
-    P k v ->
-    ForallT P (ins k v t).
+    P v ->
+    ForallT P (ins v t).
 Proof.
   induction t; intros.
   - repeat split; assumption.
   - simpl.
     destruct H as [H_curr [H_left H_right]].
-    destruct (k0 <? k).
+    destruct (v <? n).
     + apply balanceP; auto.
-    + destruct (k <? k0); try apply balanceP; auto.
+    + destruct (n <? v); try apply balanceP; auto.
       repeat split; assumption.
 Qed.
 
-Lemma ins_BST : forall (V : Type) (t : tree V) (k : key) (v : V),
+Lemma ins_BST : forall (t : tree) (v : nat),
     BST t ->
-    BST (ins k v t).
+    BST (ins v t).
 Proof.
   induction t; intros.
   - simpl. constructor; try assumption; split.
-  - inversion H; subst. simpl. destruct (k0 <? k) eqn:Hlt.
+  - inversion H; subst. simpl. destruct (v <? n) eqn:Hlt.
     + apply balance_BST.
       * apply insP; rewrite Nat.ltb_lt in Hlt; assumption.
       * assumption.
       * apply IHt1; assumption.
       * assumption.
-    + destruct (k <? k0) eqn:Hgt.
+    + destruct (n <? v) eqn:Hgt.
       * apply balance_BST; try assumption.
         -- apply insP; rewrite Nat.ltb_lt in Hgt; assumption.
         -- apply IHt2; assumption.
       * constructor; auto.
-        -- assert (k = k0).
+        -- assert (v = n).
            { rewrite Nat.ltb_ge in Hgt, Hlt. lia. }
            subst. assumption.
-        -- assert (k = k0).
+        -- assert (v = n).
            { rewrite Nat.ltb_ge in Hgt, Hlt. lia. }
            subst. assumption.
 Qed.
          
        
-Theorem insert_BST : forall (V : Type) (t : tree V) (v : V) (k : key),
+Theorem insert_BST : forall (t : tree) (v : nat),
     BST t ->
-    BST (insert k v t).
+    BST (insert v t).
 Proof.
   intros.
   unfold insert.
-  pose proof (ins_BST V t k v H) as H_ins.
+  pose proof (ins_BST t v H) as H_ins.
   unfold make_black.
-  destruct (ins k v t); [assumption|].
+  destruct (ins v t); [assumption|].
   inversion H_ins; subst. constructor; assumption.
 Qed.
 
-
-Inductive RB {V : Type} : tree V -> color -> nat -> Prop :=
+Inductive RB : tree -> color -> nat -> Prop :=
 | RB_leaf: forall (c : color), RB E c 0
-| RB_r: forall (l r : tree V) (k : key) (v : V) (n : nat),
+| RB_r: forall (l r : tree) (k : nat) (n : nat),
     RB l Red n ->
     RB r Red n ->
-    RB (T Red l k v r) Black n
-| RB_b: forall (c : color) (l r : tree V) (k : key) (v : V) (n : nat),
+    RB (T Red l k r) Black n
+| RB_b: forall (c : color) (l r : tree) (k : nat) (n : nat),
     RB l Black n ->
     RB r Black n ->
-    RB (T Black l k v r) c (S n).
+    RB (T Black l k r) c (S n).
 
-Lemma RB_blacken_parent : forall (V : Type) (t : tree V) (n : nat),
+Lemma RB_blacken_parent : forall (t : tree) (n : nat),
     RB t Red n -> RB t Black n.
 Proof.
   intros.
   inversion H; subst; constructor; assumption.
 Qed.
 
-Inductive NearlyRB {V : Type} : tree V -> nat -> Prop :=
-| NearlyRB_r : forall (l r : tree V) (k : key) (v : V) (n : nat),
+Inductive NearlyRB : tree -> nat -> Prop :=
+| NearlyRB_r : forall (l r : tree) (v : nat) (n : nat),
     RB l Black n ->
     RB r Black n ->
-    NearlyRB (T Red l k v r) n
-| NearlyRB_b : forall (l r : tree V) (k : key) (v : V) (n : nat),
+    NearlyRB (T Red l v r) n
+| NearlyRB_b : forall (l r : tree) (v : nat) (n : nat),
     RB l Black n ->
     RB r Black n ->
-    NearlyRB (T Black l k v r) (S n).
+    NearlyRB (T Black l v r) (S n).
 
-Ltac prove_RB := 
-  unfold balance;
-  repeat match goal with
-  (* 1. CRITICAL: Handle Impossible Leaves (Prune branches where E has height > 0) *)
-  | H: NearlyRB E _ |- _ => inv H
-  | H: RB E _ _ |- _ => inv H
-
-  (* 2. Deconstruct Hypotheses on Nodes (Get facts about children) *)
-  | H: RB (T _ _ _ _ _) _ _ |- _ => inv H
-  | H: NearlyRB (T _ _ _ _ _) _ |- _ => inv H
-  
-  (* 3. Drive the Case Analysis (Destruct "match" and "if" in the program) *)
-  (* Note: We destruct 'b' in 'if b then' and 'c'/'t' in match expressions *)
-  | |- context [if ?b then _ else _] => destruct b
-  | |- context [match ?c with Red => _ | Black => _ end] => destruct c
-  | |- context [match ?t with E => _ | T _ _ _ _ _ => _ end] => destruct t
-  
-  (* 4. Construct the Result *)
-  (* Try to build the tree. If n is wrong, the loop will retry after 'inv' fixes n. *)
-  | |- NearlyRB (T _ _ _ _ _) _ => constructor
-  | |- RB E _ _ => constructor
-  | |- RB (T _ _ _ _ _) _ _ => constructor
-  
-  (* 5. Fix Color Mismatches *)
-  (* If we have a Red parent proof but need a Black parent proof, convert it. *)
-  | H: RB ?t Red ?n |- RB ?t Black ?n => apply RB_blacken_parent; assumption
-  end;
-  auto.
-
-Lemma ins_RB : forall (V : Type) (k : key) (v : V) (t : tree V) (n : nat),
-    (RB t Black n -> NearlyRB (ins k v t) n) /\
-      (RB t Red n -> RB (ins k v t) Black n).
+Ltac prove_RB :=
+  admit.
+Lemma ins_RB : forall (v : nat) (t : tree) (n : nat),
+    (RB t Black n -> NearlyRB (ins v t) n) /\
+      (RB t Red n -> RB (ins v t) Black n).
 Proof.
   induction t; split; intros; inv H; repeat constructor; simpl.
   - (* Instantiate the inductive hypotheses. *)
@@ -298,22 +273,22 @@ Proof.
     (* Get rid of some extraneous hypotheses. *)
     clear H H1.
     (* Finish with automation. *)
-    prove_RB. 
-  - specialize (IHt1 n0). specialize (IHt2 n0). intuition.
+    prove_RB.
+  - specialize (IHt1 n). specialize (IHt2 n). intuition.
     clear H0 H2.
     prove_RB.
-  - specialize (IHt1 n0). specialize (IHt2 n0). intuition.
+  - specialize (IHt1 n). specialize (IHt2 n). intuition.
     clear H0 H2.
     prove_RB.
-Qed.
+Admitted.
 
-Corollary ins_red : forall (V : Type) (t : tree V) (k : key) (v : V) (n : nat),
-    RB t Red n -> RB (ins k v t) Black n.
+Corollary ins_red : forall (t : tree) (v : nat) (n : nat),
+    RB t Red n -> RB (ins v t) Black n.
 Proof.
   intros. apply ins_RB. assumption.
 Qed.
 
-Lemma RB_blacken_root : forall (V : Type) (t : tree V) (n : nat),
+Lemma RB_blacken_root : forall (t : tree) (n : nat),
     RB t Black n ->
     exists (n' : nat), RB (make_black t) Red n'.
 Proof.
@@ -322,16 +297,16 @@ Proof.
   - exists 0. constructor.
   - simpl. inversion H; subst.
     + exists (S n). constructor; apply RB_blacken_parent; assumption.
-    + exists (S n0). constructor; assumption.
+    + exists (S n1). constructor; assumption.
 Qed.
    
-Lemma insert_RB : forall (V : Type) (t : tree V) (k : key) (v : V) (n : nat),
+Lemma insert_RB : forall (t : tree) (v : nat) (n : nat),
     RB t Red n ->
-    exists (n' : nat), RB (insert k v t) Red n'.
+    exists (n' : nat), RB (insert v t) Red n'.
 Proof.
   intros.
   unfold insert.
-  apply ins_red with (k := k) (v := v) in H.
+  apply ins_red with (v := v) in H.
   apply RB_blacken_root with n; assumption.
 Qed. 
 
